--
--  lecture7.agda
--

--
--  Attendance: 55914404
--

module lecture7 where

open import prelude
open import isomorphisms
open import natural-numbers-functions
open import function-extensionality
open import List-functions 
open import Fin
open import Vector

ite-factâ‚ : (b : Bool) â†’ if b then true else false â‰¡ b
ite-factâ‚ true = refl true
ite-factâ‚ false = refl _

ite-factâ‚‚ : {X : Type} {x : X} (b : Bool) â†’ if b then x else x â‰¡ x
ite-factâ‚‚ true = refl _
ite-factâ‚‚ false = refl _

ite-factâ‚ƒ : {X : Type} {x y : X} (b : Bool)
          â†’ if b then x else y â‰¡ if not b then y else x
ite-factâ‚ƒ true = refl _
ite-factâ‚ƒ false = refl _

ite-factâ‚„ : {X : Type} {x y u v : X} (a b : Bool)
          â†’ if a then (if b then x else y) else (if b then u else v)
          â‰¡ if b then (if a then x else u) else (if a then y else v)
ite-factâ‚„ true b = refl _
ite-factâ‚„ false b = refl _

--
--  Question 2 
--

data _is-bounded-by_ : List â„• â†’ â„• â†’ Type where
  zero-bounds-[] : [] is-bounded-by zero
  stays-bounded : {b : â„•} â†’ (n : â„•) (ns : List â„•)
    â†’ ns is-bounded-by b
    â†’ n â‰¤â‚ b
    â†’ (n :: ns) is-bounded-by b
  bound-increases : {b : â„•} â†’ (n : â„•) (ns : List â„•)
    â†’ ns is-bounded-by b
    â†’ Â¬ (n â‰¤â‚ b)
    â†’ (n :: ns) is-bounded-by n

-- _is-bounded-by'_ : List â„• â†’ â„• â†’ Type
-- [] is-bounded-by' zero = ðŸ™
-- [] is-bounded-by' suc n = ðŸ˜
-- (n :: ns) is-bounded-by' b = {!!}

bounded-inductive-exampleâ‚€ : [] is-bounded-by 0
bounded-inductive-exampleâ‚€ = zero-bounds-[]

bounded-inductive-exampleâ‚ : (2 :: 1 :: [ 3 ]) is-bounded-by 3
bounded-inductive-exampleâ‚ = stays-bounded 2 (1 :: 3 :: [])
                               (stays-bounded 1 (3 :: [])
                                (bound-increases 3 [] zero-bounds-[] (Î» z â†’ z)) â‹†)
                               â‹†

bounded-inductive-exampleâ‚‚ : Â¬ ((3 :: 2 :: [ 1 ]) is-bounded-by 2)
bounded-inductive-exampleâ‚‚ (stays-bounded .3 .(2 :: [ 1 ]) _ 3â‰¤2) = 3â‰¤2

--
--  Question 3
--

Ã—-second-equation : (X Y : Type) â†’ (X âˆ” ðŸ™) Ã— Y â‰… (X Ã— Y) âˆ” Y
Ã—-second-equation X Y =
 record { bijection  = f
        ; bijectivity = record { inverse = g ; Î· = section ; Îµ = retraction } }
  where
   f : (X âˆ” ðŸ™) Ã— Y â†’ (X Ã— Y) âˆ” Y
   f (inl x , y) = inl (x , y)
   f (inr âˆ™ , y) = inr y

   g : (X Ã— Y) âˆ” Y â†’ (X âˆ” ðŸ™) Ã— Y
   g (inl (x , y)) = inl x , y
   g (inr y) = inr â‹† , y

   section : g âˆ˜ f âˆ¼ id
   section (inl x , y) = refl _
   section (inr âˆ™ , y) = refl _

   retraction : f âˆ˜ g âˆ¼ id
   retraction (inl (x , y)) = refl _
   retraction (inr y) = refl _

--
--  Question 4
--

data _âˆˆ_ {X : Type} : X â†’ List X â†’ Type where
  head-case : (x : X) (xs : List X) â†’ x âˆˆ (x :: xs)
  tail-case : (x : X) (xs : List X) â†’ x âˆˆ xs â†’ (y : X) â†’ x âˆˆ (y :: xs)

-- **Mapped membership** states that:
--  > For every list `xs` and function `f`, given any member `x` of `xs`,
--    we have that `f(x)` is also a member of the `f`-mapped list.

mapped-membership : Type â†’ Type â†’ Type
mapped-membership X Y = (xs : List X) (f : X â†’ Y) (x : X) â†’ x âˆˆ xs â†’ f x âˆˆ map f xs

--
--  Question 5
--

-- A function `f : X â†’ X` is *idempotent* if applying `f` twice yields the same
-- result as applying `f` once.

-- **Formalise** the above definition in Agda and **state** and **prove** that if
-- `f` is idempotent, then so is `map f`.

is-idempotent : (X : Type) (f : X â†’ X) â†’ Type 
is-idempotent X f = (x : X) â†’ f (f x) â‰¡ f x

-- Too strong!  This is the claim that *every* function is idempotent..
everyone-is-idempotent : (X : Type) (f : X â†’ X) (x : X) â†’ f (f x) â‰¡ f x
everyone-is-idempotent = {!!}

-- This function is *not* idempotent
suc-is-idempotent : is-idempotent â„• suc
suc-is-idempotent = {!!}

id-is-idempotent : (X : Type) â†’ is-idempotent X (Î» x â†’ x)
id-is-idempotent X x = refl x 

map-of-idempotent-function-is-idempotent : (X : Type) (f : X â†’ X) â†’ is-idempotent X f â†’ is-idempotent (List X) (map f) 
map-of-idempotent-function-is-idempotent X f is-idem-f = {!!}


