# Week 5 - Lab Sheet

```agda
{-# OPTIONS --without-K --safe #-}

module exercises.my-lab5v2 where

private
 open import prelude
 open import natural-numbers-functions hiding (_‚â§_ ; is-even ; is-odd)
 open import List-functions
 open import isomorphisms
```

We will also want to use some things from the Lab sheet of Week 4:

```agda
 open import exercises.lab4-solutions
```

## Part I: Length

In the file [List-functions.lagda.md](../List-functions.lagda.md), the
function `length` is recursively defined as follows.

```agdacode
length : {A : Type} ‚Üí List A ‚Üí ‚Ñï
length []        = 0
length (x :: xs) = 1 + length xs
```

In the following exercises we will prove some facts involving the length of
lists. In doing so, you will practise with inductive proofs.

### Exercise 1.1

Recall that we defined `map` as follows (see
[List-functions.lagda.md](../List-functions.lagda.md)).

```agdacode
map : {A B : Type} ‚Üí (A ‚Üí B) ‚Üí List A ‚Üí List B
map f []        = []
map f (x :: xs) = f x :: map f xs
```

**Prove** that `map` preserves the length of a list.

```agda
 map-preserves-length : {A B : Type} (f : A ‚Üí B) (xs : List A)
                      ‚Üí length (map f xs) ‚â° length xs
 map-preserves-length f [] = refl zero
 map-preserves-length f (x :: xs) = ap suc (map-preserves-length f xs)
```

### Exercise 1.2

Another useful fact is that the length of two concatenated lists is the sum of
their respective lengths. **Complete** the proof of this fact.

```agda
 length-of-++ : {A : Type} (xs ys : List A)
              ‚Üí length (xs ++ ys) ‚â° length xs + length ys
 length-of-++ [] ys = refl (length ys)
 length-of-++ (x :: xs) ys = ap suc (length-of-++ xs ys)
```

### Exercise 1.3

Recall `‚â§'` from Lab Sheet 4:

```agdacode
_‚â§'_ : ‚Ñï ‚Üí ‚Ñï ‚Üí Type
x ‚â§' y = Œ£ k Íûâ ‚Ñï , x + k ‚â° y
```

Similarly, we now define a list-prefix relation as follows:

```agda
 _‚âº'_ : {X : Type} ‚Üí List X ‚Üí List X ‚Üí Type
 _‚âº'_ {X} xs ys = Œ£ zs Íûâ List X , xs ++ zs ‚â° ys
```

**Prove** that the length of a prefix of a list `ys` is less than the length of
`ys`, relating the two notions above.

```agda
 length-of-prefix : {A : Type} (xs ys : List A)
                  ‚Üí xs ‚âº' ys
                  ‚Üí length xs ‚â§' length ys
 length-of-prefix [] ys (.ys , refl .ys) = ‚â§'-zero (length ys)
 length-of-prefix (x :: xs) (.x :: .(xs ++ zs)) (zs , refl .(x :: xs ++ zs))
  = ‚â§'-suc (length xs) (length (xs ++ zs)) (length-of-prefix xs (xs ++ zs) (zs , (refl (xs ++ zs))))
```

### Exercise 1.4

A nice use case of the length function is that we are now able to define safe
`head` and `tail` operations on nonempty lists.

We say that a list is *nonempty* if its length is at least 1.
```agda
 is-nonempty : {A : Type} ‚Üí List A ‚Üí Type
 is-nonempty xs = 1 ‚â§' length xs
```

We can then define `tail` as follows.
```agda
 tail : {A : Type} (xs : List A) ‚Üí is-nonempty xs ‚Üí List A
 tail (x :: xs) p = xs
```

Agda accepts this definition and does not complain about missing the `[]`-case,
because it realizes that `[]` does not satisfy `is-nonempty`.

#### Exercise 1.4a

```agda
 head : {A : Type} (xs : List A) ‚Üí is-nonempty xs ‚Üí A
 head (x :: xs) p = x
```

**Complete** the definition of `head` yourself.

#### Exercise 1.4b

```agda
 length-of-tail : {A : Type} (xs : List A) (p : 1 ‚â§' length xs)
                ‚Üí 1 + length (tail xs p) ‚â° length xs
 length-of-tail (x :: xs) p = refl (suc (length xs))
```

**Prove** that the length of a list is obtained by adding 1 to the length of the
tail.

#### Exercise 1.4c

```agda
 ‚â§'-suc-lemma : (n : ‚Ñï) ‚Üí n ‚â§' (1 + n)
 ‚â§'-suc-lemma n = 1 , +-comm n 1

 length-of-tail-decreases : {A : Type} (xs : List A) (p : 1 ‚â§' length xs)
                          ‚Üí length (tail xs p) ‚â§' length xs
 length-of-tail-decreases (x :: xs) p = ‚â§'-suc-lemma (length xs)
```

**Complete** the proof of the following lemma and use it to prove that the
length of the tail of a list is less than the length of the full list.

## Part II: Isomorphisms

Make sure you have read the [file on isomorphisms](../isomorphisms.lagda.md),
where we define ismorphisms and show that `Bool ‚âÖ ùüö`.

You will now give three more isomorphisms. In each case, you should think
about *why* and *how* each pair of types are isomorphic before attemping to
formalise the isomorphism.

### Exercise 2.1

```agda
 √ó-iso : (X Y : Type) ‚Üí X √ó Y ‚âÖ Y √ó X
 √ó-iso X Y = record { bijection = f ; bijectivity = f-is-bijection }
  where
   f : X √ó Y ‚Üí Y √ó X
   f (x , y) = y , x

   g : Y √ó X ‚Üí X √ó Y
   g (y , x) = x , y

   gf : g ‚àò f ‚àº id
   gf (x , y) = refl (x , y)

   fg : f ‚àò g ‚àº id
   fg (y , x) = refl (y , x)

   f-is-bijection : is-bijection f
   f-is-bijection = record { inverse = g ; Œ∑ = gf ; Œµ = fg }
```

**Show** that X √ó Y is isomorphic to Y √ó X using the above template.

### Exercise 2.2

```agda
 +-iso : (X Y : Type) ‚Üí X ‚àî Y ‚âÖ Y ‚àî X
 +-iso X Y = record { bijection = f ; bijectivity = f-is-bijection }
  where
   f : X ‚àî Y ‚Üí Y ‚àî X
   f (inl x) = inr x
   f (inr y) = inl y

   g : Y ‚àî X ‚Üí X ‚àî Y
   g (inl y) = inr y
   g (inr x) = inl x

   gf : g ‚àò f ‚àº id
   gf (inl x) = refl (inl x)
   gf (inr y) = refl (inr y)

   fg : f ‚àò g ‚àº id
   fg (inl y) = refl (inl y)
   fg (inr x) = refl (inr x)

   f-is-bijection : is-bijection f
   f-is-bijection = record { inverse = g ; Œ∑ = gf ; Œµ = fg }
```

### Exercise 2.3

```agda
 lists-from-vectors : {A : Type} ‚Üí List A ‚âÖ (Œ£ n Íûâ ‚Ñï , Vector A n)
 lists-from-vectors {A}
  = record { bijection = f ; bijectivity = f-is-bijection }
  where
   f : List A ‚Üí Œ£ n Íûâ ‚Ñï , Vector A n
   f [] = zero , []
   f (x :: xs) = suc (fst (f xs)) , x :: (snd (f xs))

   g : Œ£ n Íûâ ‚Ñï , Vector A n ‚Üí List A
   g (zero , []) = []
   g (suc n , x :: xs) = x :: g (n , xs)

   gf : g ‚àò f ‚àº id
   gf [] = refl []
   gf (x :: xs) = ap (x ::_) (gf xs)

   fg : f ‚àò g ‚àº id
   fg (zero , []) = refl (zero , [])
   fg ((suc n) , x :: xs) = ap (Œª (m , ys) ‚Üí suc m , x :: ys) (fg (n , xs))

   f-is-bijection : is-bijection f
   f-is-bijection = record { inverse = g ; Œ∑ = gf ; Œµ = fg }
```

**Show** that the the type `List A` is isomorphic to the type `Œ£ (Vector A)`.

(Note that this is the first question in [this question
sheet](../vector-and-list-isomorphisms.lagda.md)).

Hint: The statement of Exercise 2.3b may help you.

### Exercise 2.3b

```agda
 open _‚âÖ_

 lfv-preserves-length : {A : Type} (xs : List A)
                      ‚Üí fst (bijection lists-from-vectors xs)
                      ‚â° length xs
 lfv-preserves-length [] = refl zero
 lfv-preserves-length (x :: xs) = ap suc (lfv-preserves-length xs)
```

Notice how `bijection` extracts the function `f` you defined in
`lists-from-vectors`.

**Prove** that for any `xs : List A`, the length of `xs` is the same as the
first projection of `f xs : Œ£ (Vector A)` (where `f : ‚Ñï ‚Üí List ùüô` is as you
defined in Exercise 4a).

## Part III: Evenness

In the lecture notes, you have seen the predicates `is-even` and `is-odd`:

```agda
 is-even is-odd : ‚Ñï ‚Üí Type
 is-even x = Œ£ y Íûâ ‚Ñï , x ‚â° 2 * y
 is-odd  x = Œ£ y Íûâ ‚Ñï , x ‚â° 1 + 2 * y
```

In these exercises, we will define a Boolean-valued version of the `is-even`
predicate and prove that the two versions are _logically_ equivalent:

```agda
 check-even : ‚Ñï ‚Üí Bool
 check-even zero          = true
 check-even (suc zero)    = false
 check-even (suc (suc n)) = check-even n
```

### Exercise 3.1

First, we will have to prove two lemmas that we will use in Exercise 3.2, where
we will prove our main result.

```agda
 evenness-lemma‚ÇÅ : (n : ‚Ñï) ‚Üí is-even (2 + n) ‚Üí is-even n
 evenness-lemma‚ÇÅ n (suc k , p) = k , goal
  where
   subgoal : suc (suc n) ‚â° suc (suc (2 * k))
   subgoal = suc (suc n)       ‚â°‚ü® p ‚ü©
             suc k + suc k     ‚â°‚ü® ap suc (+-comm k (suc k)) ‚ü©
             suc ((suc k) + k) ‚àé

   goal : n ‚â° 2 * k
   goal = suc-is-injective (suc-is-injective subgoal)

 evenness-lemma‚ÇÇ : (n : ‚Ñï) ‚Üí is-even n ‚Üí is-even (2 + n)
 evenness-lemma‚ÇÇ n (k , p) = suc k , goal
  where
   goal : 2 + n ‚â° 2 * suc k
   goal = 2 + n         ‚â°‚ü® ap (suc ‚àò suc) p ‚ü©
          2 + (k + k)   ‚â°‚ü® ap suc (+-comm (suc k) k) ‚ü©
          suc k + suc k ‚àé
```

**Complete** the above proofs.

### Exercise 3.2

**Prove** that if `is-even n` then `check-even n ‚â° true`.

```agda
 even‚áícheck-even : (n : ‚Ñï) ‚Üí is-even n ‚Üí check-even n ‚â° true
 even‚áícheck-even zero even = refl true
 even‚áícheck-even (suc zero) (suc m , eq) = ùüò-elim (zero-is-not-suc (I))
   where
     I : (zero ‚â° suc (m + m))
     I = 
       zero ‚â°‚ü® ap pred eq ‚ü©
       m + suc m ‚â°‚ü® +-comm m (suc m) ‚ü©
       suc (m + m) ‚àé
       
 even‚áícheck-even (suc (suc n)) even = even‚áícheck-even n (evenness-lemma‚ÇÅ n even)
```

**Prove** that if `check-even n ‚â° true` then `is-even n`:

```agda
 check-even‚áíeven : (n : ‚Ñï) ‚Üí check-even n ‚â° true ‚Üí is-even n
 check-even‚áíeven zero even = zero , refl zero
 check-even‚áíeven (suc (suc n)) even = evenness-lemma‚ÇÇ n (check-even‚áíeven n even)
```

