# Week 9 - Lab Sheet

```agda
{-# OPTIONS  --allow-unsolved-metas --without-K --auto-inline #-}

module exercises.my-lab9 where

open import prelude
open import decidability
open import Fin
open import List-functions
open import isomorphisms
open import sorting
open import strict-total-order
```

In this lab sheet you will practice with **positions** in a list and **strict
total orders**.

## Exercise 1

Recall from the lectures that we defined a type of *positions* (or indices) for
a given list as follows.

```agdacode
Pos : {X : Type} â†’ List X â†’ Type
Pos        [] = ğŸ˜
Pos (_ :: xs) = ğŸ™ âˆ” Pos xs
```

We will consider an inductively defined version of here and prove it to be
isomorphic to `Pos`.

The inductive definition is as follows.

```agda
data Pos' {X : Type} : List X â†’ Type where
  here : {x : X} {xs : List X}
       â†’ Pos' (x :: xs)
  there : {x : X} {xs : List X}
        â†’ (p : Pos' xs) â†’ Pos' (x :: xs)
```

### Exercise 1.1

**Define** a function from `Pos xs` to `Pos' xs`.

```agda
Pos-to-Pos' : {X : Type} (xs : List X) â†’ Pos xs â†’ Pos' xs
Pos-to-Pos' (x :: [])      (inl â‹†)     = here
Pos-to-Pos' (x :: y :: xs) (inl â‹†)     = here
Pos-to-Pos' (x :: y :: xs) (inr posxs) = there (Pos-to-Pos' (y :: xs) posxs)
```

### Exercise 1.2

**Define** a function the other way, i.e. from `Pos' xs` to `Pos xs`.

```agda
Pos'-to-Pos : {X : Type} (xs : List X) â†’ Pos' xs â†’ Pos xs
Pos'-to-Pos (x :: xs) here          = inl â‹†
Pos'-to-Pos (x :: xs) (there posxs) = inr (Pos'-to-Pos xs posxs)
```

### Exercise 1.3

Using the above functions, **prove** that `Pos xs` is isomorphic to `Pos' xs`
for every list `xs`.

```agda
Pos-isomorphic-to-Pos' : {X : Type} (xs : List X) â†’ Pos xs â‰… Pos' xs
Pos-isomorphic-to-Pos' {X} xs = record { bijection = f xs ; bijectivity = f-is-bijection }
 where
  f : (xs : List X) â†’ Pos xs â†’ Pos' xs
  f xs = Pos-to-Pos' xs

  g : (xs : List X) â†’ Pos' xs â†’ Pos xs
  g xs = Pos'-to-Pos xs

  gf : (xs : List X) â†’ g xs âˆ˜ f xs  âˆ¼ id
  gf (x :: [])      (inl â‹†)     = refl (inl â‹†)
  gf (x :: y :: xs) (inl â‹†)     = refl (inl â‹†)
  gf (x :: y :: xs) (inr posxs) = ap inr (gf (y :: xs) posxs)

  fg :  (xs : List X) â†’ f xs âˆ˜ g xs âˆ¼ id
  fg (x :: [])      here          = refl here
  fg (x :: y :: xs) here          = refl here
  fg (x :: y :: xs) (there posxs) = ap there (fg (y :: xs) posxs)

  f-is-bijection : is-bijection (f xs)
  f-is-bijection = record { inverse = g xs ; Î· = gf xs; Îµ = fg xs }

```

## Exercise 2

Yet another way to define the positions is by using `Fin (length xs)`, the
inductively defined type that has exactly `length xs`-many elements.

### Exercise 2.1

**Define** the map that takes a position of `xs` and gives an element of `Fin
  (length xs)`.

```agda
Pos-to-Fin-length : {X : Type} (xs : List X) â†’ Pos xs â†’ Fin (length xs)
Pos-to-Fin-length (x :: [])      (inl â‹†)     = zero
Pos-to-Fin-length (x :: y :: xs) (inl â‹†)     = zero
Pos-to-Fin-length (x :: y :: xs) (inr posxs) = suc (Pos-to-Fin-length (y :: xs) posxs)
```

### Exercise 2.2

**Define** the map in the other direction.

```agda
Fin-length-to-Pos : {X : Type} (xs : List X) â†’ Fin (length xs) â†’ Pos xs
Fin-length-to-Pos (x :: [])      zero        = inl â‹†
Fin-length-to-Pos (x :: y :: xs) zero        = inl â‹†
Fin-length-to-Pos (x :: y :: xs) (suc finxs) = inr (Fin-length-to-Pos (y :: xs) finxs)
```

### Exercise 2.3

Using the above functions, **prove** that `Pos xs` is isomorphic to `Fin (length
xs)` for every list `xs`.

```agda
Pos-isomorphic-to-Fin-length : {X : Type} (xs : List X)
                             â†’ Pos xs â‰… Fin (length xs)
Pos-isomorphic-to-Fin-length {X} xs = record { bijection = f xs ; bijectivity = f-is-bijection }
 where
  f : (xs : List X) â†’ Pos xs â†’ Fin (length xs)
  f = Pos-to-Fin-length

  g : (xs : List X) â†’ Fin (length xs) â†’ Pos xs
  g = Fin-length-to-Pos

  gf : (xs : List X) â†’ g xs âˆ˜ f xs âˆ¼ id
  gf (x :: [])      (inl â‹†)     = refl (inl â‹†)
  gf (x :: y :: xs) (inl â‹†)     = refl (inl â‹†)
  gf (x :: y :: xs) (inr posxs) = ap inr (gf (y :: xs) posxs)

  fg : (xs : List X) â†’ f xs âˆ˜ g xs âˆ¼ id
  fg (x :: [])      zero        = refl zero
  fg (x :: y :: xs) zero        = refl zero
  fg (x :: y :: xs) (suc finxs) = ap suc (fg (y :: xs) finxs)

  f-is-bijection : is-bijection (f xs)
  f-is-bijection = record { inverse = g xs ; Î· = gf xs ; Îµ = fg xs }

```

## Exercise 3

**Prove** that if `X` and `Y` have decidable equality, then so does their
cartesian product `X Ã— Y`.

```agda
flip : {X Y : Type} â†’ X Ã— Y â†’ Y Ã— X
flip (x , y) = y , x

pair-lemma1 : {X Y : Type}(xâ‚ xâ‚‚ : X)(yâ‚ yâ‚‚ : Y) â†’ Â¬ (xâ‚ â‰¡ xâ‚‚) â†’ Â¬ ((xâ‚ , yâ‚) â‰¡ (xâ‚‚ , yâ‚‚))
pair-lemma1 xâ‚ xâ‚‚ yâ‚ yâ‚‚ Â¬eq eqpair = ğŸ˜-elim (Â¬eq (ap fst eqpair))

pair-lemma2 : {X Y : Type}(xâ‚ xâ‚‚ : X)(yâ‚ yâ‚‚ : Y) â†’ Â¬ (yâ‚ â‰¡ yâ‚‚) â†’ Â¬ ((xâ‚ , yâ‚) â‰¡ (xâ‚‚ , yâ‚‚))
pair-lemma2 xâ‚ xâ‚‚ yâ‚ yâ‚‚ Â¬eq eqpair = ğŸ˜-elim (Â¬eq (ap snd eqpair))

pair-lemma3 : {X Y : Type}(xâ‚ xâ‚‚ : X)(yâ‚ yâ‚‚ : Y) â†’ xâ‚ â‰¡ xâ‚‚ â†’ yâ‚ â‰¡ yâ‚‚ â†’ (xâ‚ , yâ‚) â‰¡ (xâ‚‚ , yâ‚‚)
pair-lemma3 x .x y .y (refl .x) (refl .y) = refl (x , y)

Ã—-has-decidable-equality : {X Y : Type}
                         â†’ has-decidable-equality X
                         â†’ has-decidable-equality Y
                         â†’ has-decidable-equality (X Ã— Y)
Ã—-has-decidable-equality deceqx deceqy (xâ‚ , yâ‚) (xâ‚‚ , yâ‚‚) = I (deceqx xâ‚ xâ‚‚) (deceqy yâ‚ yâ‚‚)
  where
    I : is-decidable (xâ‚ â‰¡ xâ‚‚) â†’ is-decidable (yâ‚ â‰¡ yâ‚‚) â†’ is-decidable ((xâ‚ , yâ‚) â‰¡ (xâ‚‚ , yâ‚‚))
    I (inl eqx)  (inl eqy)  = inl (pair-lemma3 xâ‚ xâ‚‚ yâ‚ yâ‚‚ eqx eqy)
    I (inl eqx)  (inr Â¬eqy) = inr (pair-lemma2 xâ‚ xâ‚‚ yâ‚ yâ‚‚ Â¬eqy)
    I (inr Â¬eqx) _          = inr (pair-lemma1 xâ‚ xâ‚‚ yâ‚ yâ‚‚ Â¬eqx)
```

**Conclude** that `â„• Ã— â„•` has decidable equality.

```agda
â„•Â² : Type
â„•Â² = â„• Ã— â„•

â„•Â²-has-decidable-equality : has-decidable-equality â„•Â²
â„•Â²-has-decidable-equality = Ã—-has-decidable-equality â„•-has-decidable-equality â„•-has-decidable-equality
```

## Exercise 4

The *lexicographical order* on `â„•Â²` is defined as: `(n , m) < (n' , m')`
precisely when (`n < n'`) or (`n = n'` and `m < m'`).

So, for example, `(3 , 19) < (5, 2)` and `(7 , 3) < (7 , 4)`, but `Â¬ (11 , 4) <
(11 , 1)` and `Â¬ (5 , 1) < (4 , 3)`.

We are going to prove that the lexicographical order is a strict total order on
`â„•Â²`.

### Exercise 4.1

**Translate** the definition of the lexicographical order to Agda.

```agda
_<â‚—_ : â„•Â² â†’ â„•Â² â†’ Type
(zero , m)     <â‚— (zero , zero)     = ğŸ˜
(zero , zero)  <â‚— (zero , suc m')   = ğŸ™
(zero , suc m) <â‚— (zero , suc m')   = (zero , m) <â‚— (zero , m')
(zero , m)     <â‚— (suc n' , m')     = ğŸ™
(suc n , m)    <â‚— (zero , m')       = ğŸ˜
(suc n , m)    <â‚— (suc n' , m')     = (n , m) <â‚— (n' , m')
```

### Exercise 4.2

**Prove** that the lexicographical order is irreflexive.

```agda
<â‚—-is-irreflexive : (p : â„•Â²) â†’ Â¬ (p <â‚— p)
<â‚—-is-irreflexive (zero , suc m) p< = <â‚—-is-irreflexive (zero , m) p<
<â‚—-is-irreflexive (suc n , m) p< = <â‚—-is-irreflexive (n , m) p<
```

### Exercise 4.3

**Prove** that the lexicographical order is transitive.

```agda
<â‚—-is-transitive : {p q r : â„•Â²} â†’ p <â‚— q â†’ q <â‚— r â†’ p <â‚— r
<â‚—-is-transitive {zero , zero}     {zero , suc sndâ‚‚} {zero , suc sndâ‚ƒ} p<q q<r = â‹†
<â‚—-is-transitive {zero , zero}     {zero , suc sndâ‚‚} {suc fstâ‚ƒ , sndâ‚ƒ} p<q q<r = â‹†
<â‚—-is-transitive {zero , suc sndâ‚} {zero , suc sndâ‚‚} {zero , suc sndâ‚ƒ} p<q q<r = <â‚—-is-transitive {zero , sndâ‚} {zero , sndâ‚‚} {zero , sndâ‚ƒ} p<q q<r
<â‚—-is-transitive {zero , suc sndâ‚} {zero , suc sndâ‚‚} {suc fstâ‚ƒ , sndâ‚ƒ} p<q q<r = â‹†
<â‚—-is-transitive {zero , zero} {suc fstâ‚ , zero} {suc fstâ‚‚ , sndâ‚} p<q q<r = â‹†
<â‚—-is-transitive {zero , zero} {suc fstâ‚ , suc sndâ‚} {suc fstâ‚‚ , sndâ‚‚} p<q q<r = â‹†
<â‚—-is-transitive {zero , suc sndâ‚} {suc fstâ‚ , zero} {suc fstâ‚‚ , sndâ‚‚} p<q q<r = â‹†
<â‚—-is-transitive {zero , suc sndâ‚} {suc fstâ‚ , suc sndâ‚‚} {suc fstâ‚‚ , sndâ‚ƒ} p<q q<r = â‹†
<â‚—-is-transitive {suc fstâ‚ , sndâ‚} {zero , sndâ‚‚}     {zero , sndâ‚ƒ}     p<q q<r = p<q
<â‚—-is-transitive {suc fstâ‚ , sndâ‚} {suc fstâ‚‚ , sndâ‚‚} {zero , sndâ‚ƒ}     p<q q<r = q<r
<â‚—-is-transitive {suc fstâ‚ , sndâ‚} {suc fstâ‚‚ , sndâ‚‚} {suc fstâ‚ƒ , sndâ‚ƒ} p<q q<r = <â‚—-is-transitive {fstâ‚ , sndâ‚} {fstâ‚‚ , sndâ‚‚} {fstâ‚ƒ , sndâ‚ƒ} p<q q<r
```

### Exercise 4.4

**Prove** that the lexicographical is connected.

```agda
<â‚—-is-connected : {p q : â„•Â²} â†’ Â¬ (p â‰¡ q) â†’ (p <â‚— q) âˆ” (q <â‚— p)
<â‚—-is-connected {zero , zero} {zero , zero} Â¬peqq = ğŸ˜-elim (Â¬peqq (refl (zero , zero)))
<â‚—-is-connected {zero , zero} {zero , suc sndâ‚‚} Â¬peqq = inl â‹†
<â‚—-is-connected {zero , suc sndâ‚} {zero , zero} Â¬peqq = inr â‹†
<â‚—-is-connected {zero , suc sndâ‚} {zero , suc sndâ‚‚} Â¬peqq = <â‚—-is-connected {zero , sndâ‚} {zero , sndâ‚‚} (Î» prf â†’ Â¬peqq (ap (Î» x â†’ zero , suc (snd x)) prf))
<â‚—-is-connected {zero , zero} {suc fstâ‚ , zero} x = inl â‹†
<â‚—-is-connected {zero , zero} {suc fstâ‚ , suc sndâ‚} x = inl â‹†
<â‚—-is-connected {zero , suc sndâ‚} {suc fstâ‚ , zero} x = inl â‹†
<â‚—-is-connected {zero , suc sndâ‚} {suc fstâ‚ , suc sndâ‚‚} x = inl â‹†
<â‚—-is-connected {suc fstâ‚ , sndâ‚} {zero , zero} Â¬peqq = inr â‹†
<â‚—-is-connected {suc fstâ‚ , sndâ‚} {zero , suc sndâ‚‚} Â¬peqq = inr â‹†
<â‚—-is-connected {suc fstâ‚ , sndâ‚} {suc fstâ‚‚ , sndâ‚‚} Â¬peqq = <â‚—-is-connected {fstâ‚ , sndâ‚} {fstâ‚‚ , sndâ‚‚} (Î» prf â†’ Â¬peqq (ap (Î» p â†’ suc (fst p) , snd p) prf))
```

### Exercise 4.5

**Conclude** that the lexicographical order is a strict total order on `â„•Â²`.

```agda
strict-total-order-on-â„•Â² : StrictTotalOrder â„•Â²
strict-total-order-on-â„•Â² = record
                             { _<_ = _<â‚—_
                             ; irreflexive = <â‚—-is-irreflexive
                             ; transitive = Î» {p} {q} {r} â†’ <â‚—-is-transitive {p} {q} {r}
                             ; connected = <â‚—-is-connected
                             ; decidable = â„•Â²-has-decidable-equality
                             }
```

## Exercise 5

In the lectures, a type f strict total order was introduced. Similarly, we can
also introduce a type of *non-strict total orders*.

For example, the type of natural numbers with `â‰¤` is an example of a non-strict
total order.

```agda
record NonStrictTotalOrder (X : Type) : Typeâ‚ where
 field
  _â‰¤_ : X â†’ X â†’ Type
  decidable : has-decidable-equality X
  reflexive : (x : X) â†’ x â‰¤ x
  transitive : {x y z : X} â†’ x â‰¤ y â†’ y â‰¤ z â†’ x â‰¤ z
  antisymmetric : {x y : X} â†’ x â‰¤ y â†’ y â‰¤ x â†’ x â‰¡ y
  strongly-connected : (x y : X) â†’ (x â‰¤ y) âˆ” (y â‰¤ x)
```

Now let's assume that we are given a *strict* total order. We make this
assumption using a module, which means it will be available to you in the code
below.

```agda
module _
        {X : Type}
        (sto : StrictTotalOrder X)
       where

 open StrictTotalOrder sto
```

We can define the order `â‰¤` from the strict total order `<` on `X` as follows.

```agda
 _â‰¤_ : X â†’ X â†’ Type
 x â‰¤ y = (y â‰¡ x) âˆ” (x < y)
```

Notice how `â‰¤` was (implicitly) used in the definition of `Sorted` given in
[strict-total-order.lagda.md](../strict-total-order.lagda.md#sorted-lists).

### Exercise 5.1

**Prove** the following facts about `â‰¤`.

```agda
 <-to-â‰¤ : {x y : X} â†’ x < y â†’ x â‰¤ y
 <-to-â‰¤ x<y = inr x<y

 â‰¤-is-reflexive : (x : X) â†’ x â‰¤ x
 â‰¤-is-reflexive x = inl (refl x)
```

### Exercise 5.2

Using transitivity of `<`, **prove** a lemma and that `â‰¤` is transitive.

```agda
 <-â‰¤-trans : {x y z : X} â†’ x < y â†’ y â‰¤ z â†’ x â‰¤ z
 <-â‰¤-trans {x} {y} {.y} x<y (inl (refl .y)) = inr x<y
 <-â‰¤-trans {x} {y} {z}  x<y (inr y<z)       = inr (transitive x<y y<z)

 â‰¤-is-transitive : {x y z : X} â†’ x â‰¤ y â†’ y â‰¤ z â†’ x â‰¤ z
 â‰¤-is-transitive {x} {.x} {z} (inl (refl .x)) yâ‰¤z = yâ‰¤z
 â‰¤-is-transitive {x} {y}  {z} (inr x<y)       yâ‰¤z = <-â‰¤-trans x<y yâ‰¤z
```

### Exercise 5.3

**Prove** antisymmetry of `â‰¤`.

```agda
 lt-lemma : (x y : X) â†’ x < y â†’ Â¬ (y < x)
 lt-lemma x y x<y y<x = irreflexive x (transitive x<y y<x) 

 â‰¤-is-antisymmetric : {x y : X} â†’ x â‰¤ y â†’ y â‰¤ x â†’ x â‰¡ y
 â‰¤-is-antisymmetric (inl yâ‰¡x) _ = sym yâ‰¡x
 â‰¤-is-antisymmetric (inr _) (inl xâ‰¡y) = xâ‰¡y
 â‰¤-is-antisymmetric {x} {y} (inr x<y) (inr y<x) = ğŸ˜-elim (irreflexive x (transitive x<y y<x))
```

### Exercise 5.4

**Show** that `â‰¤` is strongly connected.

```agda
 â‰¤-is-strongly-connected : (x y : X) â†’ (x â‰¤ y) âˆ” (y â‰¤ x)
 â‰¤-is-strongly-connected x y = I (decidable x y)
  where
   I : is-decidable (x â‰¡ y) â†’ (x â‰¤ y) âˆ” (y â‰¤ x)
   I (inl xâ‰¡y)  = inr (inl xâ‰¡y)
   I (inr Â¬xâ‰¡y) = II (connected Â¬xâ‰¡y)
     where
       II : (x < y) âˆ” (y < x) â†’ (x â‰¤ y) âˆ” (y â‰¤ x)
       II (inl x<y) = inl (inr x<y)
       II (inr y<x) = inr (inr y<x)
```

### Exercise 5.5

Finally, **complete** the definition of the non-strict total order on `X`.

```agda
 non-strict-total-order-from-strict-total-order : NonStrictTotalOrder X
 non-strict-total-order-from-strict-total-order = record
  { _â‰¤_ = _â‰¤_
  ; decidable = decidable
  ; reflexive = â‰¤-is-reflexive
  ; transitive = â‰¤-is-transitive
  ; antisymmetric = â‰¤-is-antisymmetric
  ; strongly-connected = â‰¤-is-strongly-connected
  }
```
